Port SimplePingProtocol to use safe protocol module

protocols/SimplePingProtocol.v
@@ -22,16 +22,15 @@ Require Import
         MyPrelude
         Maps
         Messages
-        (* MessageEq *)
         Common
         Keys
-        (* KeysTheory *)
         Automation
         Tactics
         Simulation
         AdversaryUniverse
         UniverseEqAutomation
-        ProtocolAutomation.
+        ProtocolAutomation
+        SafeProtocol.
 
 Require IdealWorld RealWorld.
 
@@ -85,13 +84,6 @@ Section IdealProtocol.
          (* user B *)
          ( m <- @Return (Message Nat) (Content n)
          ; ret (extractContent m)).
-
-  Definition ideal_univ_done n :=
-    mkiU ($0 $+ (CH__A2B, []))
-         (* user A *)
-         (Return n)
-         (* user B *)
-         (Return n).
 
 End IdealProtocol.
 
@@ -191,215 +183,254 @@ Section RealProtocol.
       -> RSimplePing (peel_adv U__r) (ideal_univ_recd1 n)
   .
 
-End RealProtocol.
+  Lemma Sent1' : forall U__r U__i cs mycs1 mycs2 cur_n1 cur_n2 n cid1 non1 adv,
+      ~^* (real_univ_sent1 n cs mycs1 mycs2 cur_n1 cur_n2 cid1 non1 adv) U__r
+      -> @lameAdv Unit tt adv
+      -> U__i = ideal_univ_sent1 n
+      -> RSimplePing (peel_adv U__r) U__i.
+  Proof. intros; subst; eapply Sent1; eauto. Qed.
+  
+  Lemma Recd1' : forall U__r U__i cs mycs1 mycs2 cur_n1 cur_n2 n cid1 non1 adv,
+      ~^* (real_univ_recd1 n cs mycs1 mycs2 cur_n1 cur_n2 cid1 non1 adv) U__r
+      -> @lameAdv Unit tt adv
+      -> U__i = ideal_univ_recd1 n
+      -> RSimplePing (peel_adv U__r) U__i.
+  Proof. intros; subst; eapply Recd1; eauto. Qed.
 
-Hint Constructors
-     RSimplePing.
+End RealProtocol.
 
 Hint Unfold
      A B PERMS__a PERMS__b
      real_univ_start real_univ_sent1 real_univ_recd1 mkrU
-     ideal_univ_start ideal_univ_sent1 ideal_univ_recd1 ideal_univ_done mkiU : constants.
+     ideal_univ_start ideal_univ_sent1 ideal_univ_recd1 mkiU : constants.
 
 Import SimulationAutomation.
+
+(* Hint Constructors *)
+(*      RSimplePing. *)
+Hint Extern 1 (RSimplePing (RealWorld.peel_adv _) _) =>
+  simpl; simpl_real_users_context; simpl_ideal_users_context; simpl;
+   ( (eapply Start  ; solve [ eauto ])
+   || (eapply Recd1' ; solve [ eauto ])
+   || (eapply Sent1' ; solve [ eauto ]) ).
 
 Hint Extern 0 (~^* _ _) =>
  progress(unfold real_univ_start, real_univ_sent1, real_univ_recd1, mkrU; simpl).
 Hint Extern 1 (RSimplePing (RealWorld.buildUniverse _ _ _ _ _ _) _) => unfold RealWorld.buildUniverse; simpl.
-Hint Extern 1 (RSimplePing (RealWorld.peel_adv _) _) => unfold RealWorld.peel_adv; simpl.
 
 Hint Extern 0 (IdealWorld.lstep_universe _ _ _) =>
- progress(unfold ideal_univ_start, ideal_univ_sent1, ideal_univ_recd1, ideal_univ_done, mkiU; simpl).
+ progress(unfold ideal_univ_start, ideal_univ_sent1, ideal_univ_recd1, mkiU; simpl).
 
 (* Hint Extern 1 (IdealWorld.lstep_universe _ _ _) => single_step_ideal_universe; eauto 2; econstructor. *)
 Hint Extern 1 (PERMS__a $? _ = _) => unfold PERMS__a.
 Hint Extern 1 (PERMS__b $? _ = _) => unfold PERMS__b.
 
-Section FeebleSimulates.
+Hint Extern 1 (istepSilent ^* _ _) =>
+unfold ideal_univ_start, ideal_univ_sent1, ideal_univ_recd1, mkiU; simpl;
+  repeat (ideal_single_silent_multistep A);
+  repeat (ideal_single_silent_multistep B); solve_refl.
 
-  Hint Extern 0 (istepSilent ^* _ _) =>
-    progress(unfold ideal_univ_start, ideal_univ_sent1, ideal_univ_recd1, ideal_univ_done, mkiU; simpl).
-  Hint Extern 1 (istepSilent ^* _ _) =>
-    unfold ideal_univ_start, ideal_univ_sent1, ideal_univ_recd1, ideal_univ_done, mkiU; simpl;
-    repeat (ideal_single_silent_multistep A);
-    repeat (ideal_single_silent_multistep B); solve_refl.
 
-  
-  Lemma rsimpleping_silent_simulates :
-    simulates_silent_step (@lameAdv Unit tt) RSimplePing.
+Module SimplePingProtocolSecure <: SafeProtocol.
+  Definition A := Nat.
+  Definition B := Unit.
+
+  Definition U__i := ideal_univ_start.
+  Definition U__r := real_univ_start $0 [] [] 0 0 startAdv.
+
+  Definition b := tt.
+  Definition R := RSimplePing.
+
+  Lemma U_good : @universe_starts_sane _ Unit b U__r.
   Proof.
-    unfold simulates_silent_step.
-
-    time (
-        intros * R UOK AOK LAME * STEP;
-        clear UOK AOK;
-        invert R;
-        destruct U__r0; destruct U__r; simpl in *; subst;
-        churn; simpl_real_users_context;
-        [> eexists; split; swap 1 2; eauto 12 ..]
-      ).
+    unfold b, U__r, real_univ_start, mkrU, startAdv.
+    unfold universe_starts_sane; simpl.
+    repeat (apply conj); intros; eauto.
+    - solve_perm_merges; eauto.
+    - econstructor.
+    - unfold AdversarySafety.keys_honest, KEYS; rewrite Forall_natmap_forall; intros.
+      econstructor; simpl.
+      rewrite !findUserKeys_add_reduce, findUserKeys_empty_is_empty; eauto.
+      solve_perm_merges.
+    - unfold lameAdv; simpl; eauto.
   Qed.
 
-  Lemma rsimpleping_loud_simulates :
-    simulates_labeled_step (@lameAdv Unit tt) RSimplePing.
+  Lemma R_silent_simulates : simulates_silent_step (@lameAdv Unit b) R.
   Proof.
-    unfold simulates_labeled_step.
+    unfold b, R, simulates_silent_step.
 
-    time (
-        intros * R UOK AOK LAME * STEP;
-        clear UOK AOK;
-        invert R;
-        destruct U__r0; destruct U__r; simpl in *; subst;
-        churn;
-        [> do 3 eexists;
-         repeat (apply conj);
-         swap 3 4; swap 2 3; swap 1 2;
-         simpl; clean_map_lookups; eauto 12 ..]
-      ).
-
-  Qed.
-
-  Lemma rsimpleping_honest_actions_safe :
-    honest_actions_safe Unit RSimplePing.
-  Proof.
-    unfold honest_actions_safe; intros.
-    clear H0 H1.
-    inversion H; clear H;
+    intros * R UOK AOK LAME * STEP;
+      clear UOK AOK;
+      invert R;
       destruct U__r0; destruct U__r; simpl in *; subst.
 
-    - churn;
-        [> solve_honest_actions_safe; clean_map_lookups; eauto 8 .. ].
+    - churn; simpl_real_users_context.
+      + eexists; split; [ solve_refl | ]; eauto 12.
+      + eexists; split; [ solve_refl | ]; eauto 12.
+      + eexists; split; [ solve_refl | ]; eauto 12.
+      + eexists; split; [ solve_refl | ]; eauto 12.
+
+    - churn; simpl_real_users_context.
+      + eexists; split; [ solve_refl | ]; eauto 12.
+        
+    - churn; simpl_real_users_context.
+ 
+      + eexists; split; [ solve_refl | ]; eauto 12.
+      + eexists; split; [ solve_refl | ]; eauto 12.
+      + eexists; split; [ solve_refl | ]; eauto 12.
+      + eexists; split; [ solve_refl | ]; eauto 12.
+      + eexists; split; [ solve_refl | ]; eauto 12.
+      + eexists; split; [ solve_refl | ]; eauto 12.
+      + eexists; split; [ solve_refl | ]; eauto 12.
+      + eexists; split; [ solve_refl | ]; eauto 12.
+      + eexists; split; [ solve_refl | ]; eauto 12.
+      + eexists; split; [ solve_refl | ]; eauto 12.
+      + eexists; split; [ solve_refl | ]; eauto 12.
+      + eexists; split; [ solve_refl | ]; eauto 12.
+      + eexists; split; [ solve_refl | ]; eauto 12.
+
+    (* Time ( *)
+    (*     intros * R UOK AOK LAME * STEP; *)
+    (*     clear UOK AOK; *)
+    (*     invert R; *)
+    (*     destruct U__r0; destruct U__r; simpl in *; subst; *)
+    (*     churn; simpl_real_users_context; *)
+    (*     [> eexists; split; swap 1 2; eauto 12 ..] *)
+    (*   ). *)
+  Qed.
+
+  Lemma R_loud_simulates : simulates_labeled_step (@lameAdv Unit b) R.
+  Proof.
+    unfold b, R, simulates_labeled_step.
+
+    intros * R UOK AOK LAME * STEP;
+      clear UOK AOK;
+      invert R;
+      destruct U__r0; destruct U__r; simpl in *; subst.
+
+    - churn; simpl_real_users_context; simpl.
+
+      + do 3 eexists;
+          repeat (apply conj); eauto 12.
+
+    - churn; simpl_real_users_context.
+      
+      + do 3 eexists;
+          repeat (apply conj); eauto.
+
+      + do 3 eexists;
+          repeat (apply conj); eauto 12.
+
+    - churn; simpl_real_users_context.
+
+    (* time *)
+    (*   (intros; *)
+    (*    invert H; *)
+    (*    try destruct U__r0; try destruct U__r; simpl in *; subst; *)
+    (*    churn; *)
+    (*    simpl_real_users_context; *)
+    (*    (* autorewrite with simpl_univ; *) *)
+    (*    (* simpl; *) *)
+    (*    (do 3 eexists; *)
+    (*     repeat (apply conj); *)
+    (*     swap 3 4; swap 2 3; swap 1 2; [ .. | admit (* action matches predicate *)]; *)
+    (*     simpl; clean_map_lookups; *)
+    (*     eauto; eauto 12)). *)
+  Qed.
+  
+  Lemma R_honest_actions_safe : honest_actions_safe B R.
+  Proof.
+    unfold B, R, honest_actions_safe; intros.
+    clear H0 H1.
+    
+    inversion H; clear H;
+      destruct U__r0; destruct U__r; simpl in *; subst;
+        try match goal with
+            | [ H : ~ In ?k KEYS |- _ ] => 
+              rewrite not_find_in_iff in H;
+              solve_concrete_maps; solve_perm_merges
+            end.
 
     - churn;
-        [> solve_honest_actions_safe; clean_map_lookups; eauto 8 .. ].
+        [> solve_honest_actions_safe; eauto 8 ..].
       
     - churn;
-        [> solve_honest_actions_safe; clean_map_lookups; eauto 8 .. ].
+        [> solve_honest_actions_safe; eauto 8 ..].
+
+    - churn;
+        [> solve_honest_actions_safe; eauto 8 ..].
 
       Unshelve.
-      all: eauto.
+      all: auto.
   Qed.
 
-  (* Timings:
-   *
-   * --------------------------------------------------------------
-   * --------------------------------------------------------------
-   *)
-
-  Hint Resolve
-       rsimpleping_silent_simulates
-       rsimpleping_loud_simulates
-       rsimpleping_honest_actions_safe.
-
-  Lemma univ_ok_start :
-    forall adv,
-      @lameAdv Unit tt adv
-      -> universe_ok (real_univ_start $0 [] [] 0 0 adv).
+  Lemma univ_ok_start : universe_ok U__r.
   Proof.
-    unfold real_univ_start; econstructor; eauto.
+    unfold real_univ_start, U__r; econstructor; eauto.
   Qed.
 
-      Lemma merge_perms_true_either_true :
-      forall ks1 ks2 k_id,
-        ks1 $? k_id = Some true \/ ks2 $? k_id = Some true
-        -> ks1 $k++ ks2 $? k_id = Some true.
-    Proof.
-      intros; split_ors; solve_perm_merges.
-    Qed.
-
-    Hint Resolve merge_perms_true_either_true.
-
-
-  Lemma adv_univ_ok_start :
-    forall adv U__r honestk,
-      U__r = real_univ_start $0 [] [] 0 0 adv
-      -> honestk = RealWorld.findUserKeys U__r.(RealWorld.users)
-      -> @lameAdv Unit tt adv
-      -> adv.(RealWorld.key_heap) = $0
-      -> adv.(RealWorld.msg_heap) = []
-      -> adv.(RealWorld.c_heap) = []
-      -> adv_universe_ok (real_univ_start $0 [] [] 0 0 adv).
+  Lemma adv_univ_ok_start : adv_universe_ok U__r.
   Proof.
-    intros; unfold lameAdv in *;
-    unfold real_univ_start
-         , adv_universe_ok
-         , keys_and_permissions_good
-         , permission_heap_good.
-         
-    simpl; intuition (subst; eauto).
+    unfold adv_universe_ok, U__r; eauto.
+    unfold keys_and_permissions_good.
+    pose proof (adversary_is_lame_adv_univ_ok_clauses U_good).
+
+    intuition eauto;
+      unfold real_univ_start, mkrU in *; simpl in *.
 
     - unfold KEYS in *; solve_simple_maps; eauto.
-    - rewrite Forall_natmap_forall; intros;
-        unfold A__keys, B__keys, KEYS in *;
-        simpl in *; solve_simple_maps;
-          simpl in *; solve_simple_maps;
-            eauto.
-    - rewrite H2 in H5; clean_map_lookups.
+    - rewrite Forall_natmap_forall; intros.
+      solve_simple_maps; simpl;
+        unfold permission_heap_good, KEYS, A__keys, B__keys; intros;
+          solve_simple_maps; eauto.
 
     - unfold user_cipher_queues_ok.
       rewrite Forall_natmap_forall; intros.
-      cases (A ==n k); cases (B ==n k); subst; clean_map_lookups; simpl in *; econstructor; eauto.
-
-    - unfold message_queues_ok.
-      rewrite Forall_natmap_forall; intros.
-      cases (A ==n k); cases (B ==n k); subst; clean_map_lookups; simpl in *; econstructor; eauto.
-
-    - unfold adv_cipher_queue_ok.
-      rewrite Forall_forall; intros.
-      rewrite H4 in H; simpl in H; contradiction.
-
-    - unfold adv_message_queue_ok.
-      rewrite Forall_forall; intros.
-      rewrite H3 in H; simpl in H; contradiction.
-
-    - unfold adv_no_honest_keys; intros.
-      rewrite !findUserKeys_add_reduce, findUserKeys_empty_is_empty; eauto.
-      unfold A__keys , B__keys; destruct (k_id ==n KID1); subst; solve_perm_merges.
-      + right; right.
-        rewrite H2; split; clean_map_lookups; eauto.
-      + left; apply merge_perms_adds_no_new_perms; eauto.
+      cases (SimplePingProtocol.A ==n k); cases (SimplePingProtocol.B ==n k);
+        subst; clean_map_lookups; simpl in *; econstructor; eauto.
 
     - unfold honest_nonces_ok; intros.
       unfold honest_nonce_tracking_ok.
 
-      destruct (u_id ==n A); destruct (u_id ==n B);
-        destruct (rec_u_id ==n A); destruct (rec_u_id ==n B);
-          unfold A in *; unfold B in *;
-            subst; try contradiction; try discriminate;
-              clean_map_lookups; eauto; simpl; repeat (apply conj); intros;
-                clean_map_lookups; eauto.
+      destruct (u_id ==n SimplePingProtocol.A); destruct (u_id ==n SimplePingProtocol.B);
+        destruct (rec_u_id ==n SimplePingProtocol.A); destruct (rec_u_id ==n SimplePingProtocol.B);
+          subst; try contradiction; try discriminate; clean_map_lookups; simpl;
+            repeat (apply conj); intros; clean_map_lookups; eauto.
 
     - unfold honest_users_only_honest_keys; intros.
-      destruct (u_id ==n A); destruct (u_id ==n B);
+      destruct (u_id ==n SimplePingProtocol.A);
+        destruct (u_id ==n SimplePingProtocol.B);
         subst;
         simpl in *;
         clean_map_lookups;
         rewrite !findUserKeys_add_reduce, findUserKeys_empty_is_empty;
         eauto;
-        simpl in *.
-
-      + unfold A__keys in H0; destruct (KID1 ==n k_id); subst; clean_map_lookups; eauto.
-      + unfold B__keys in H0; destruct (KID1 ==n k_id); subst; clean_map_lookups; eauto.
+        simpl in *;
+        solve_perm_merges;
+        solve_concrete_maps;
+        solve_simple_maps;
+        eauto.
   Qed.
-
-  Hint Resolve
-       univ_ok_start
-       adv_univ_ok_start.
-
-  Theorem base_pingpong_refines_ideal_pingpong :
-    forall adv U__r honestk,
-      U__r = real_univ_start $0 [] [] 0 0 adv
-      -> honestk = RealWorld.findUserKeys U__r.(RealWorld.users)
-      -> @lameAdv Unit tt adv
-      -> RealWorld.key_heap adv = $0
-      -> RealWorld.msg_heap adv = []
-      -> RealWorld.c_heap adv = []
-      -> adv_message_queue_ok U__r.(RealWorld.users) U__r.(RealWorld.all_ciphers) U__r.(RealWorld.all_keys) adv.(RealWorld.msg_heap)
-      -> adv_no_honest_keys honestk adv.(RealWorld.key_heap)
-      -> refines (@lameAdv Unit tt) U__r ideal_univ_start.
+  
+  
+  Lemma universe_starts_safe : R (RealWorld.peel_adv U__r) U__i /\ universe_ok U__r /\ adv_universe_ok U__r.
   Proof.
-    exists RSimplePing; unfold simulates.
-    intuition (subst; eauto).
+    repeat (simple apply conj);
+      eauto using univ_ok_start, adv_univ_ok_start.
+
+    pose proof U_good;
+      unfold universe_starts_sane, adversary_is_lame in *;
+      split_ands;
+      unfold R;
+      unfold U__r in *;
+      eapply Start;
+      eauto.
   Qed.
 
-End FeebleSimulates.
+End SimplePingProtocolSecure.
+
+(* Timings:
+ *
+ * --------------------------------------------------------------
+ * --------------------------------------------------------------
+ *)
